Main.fst
@@ -2,23 +2,36 @@ module Main
 
 open FStar.String
 open FStar.IO
-open FormulaT
+open Utils
+// open FormulaT
+open FStar.List.Tot.Base
 
 
-let main = let f0 = Var 0 in
-           let f1 = Var 1 in
-           let f2 = Var 2 in
-           let f3 = Var 3 in 
-           let var_for_rule_0 = DImplies f0 f1 in
-           let var_for_rule_1 = Implies f0 f1 in
-           let var_for_rule_2 = Or f0 (And f1 f2) in
-           let var_for_rule_3 = Or (And f1 f2) (DImplies f0 f1) in
-           let var_for_rule_5 = Or f0 (Or f1 f2) in
-           let var_for_rule_6 = And f0 (And f1 f2) in
-           let var_for_rule_7 = Not (And f0 f1) in
-           let var_for_rule_8 = Not (Or f0 f1) in
-           let var_for_rule_9 = Not (Not f0) in
-           let test_formula = DImplies (Or f1 f2) f0 in
-           let out1 = FStar.Printf.sprintf "%s\n" (pretty_print test_formula) in
-              print_string out1;
-              print_string (pretty_print var_for_rule_3)
+let rec list_int_to_list_string (a:list int) : list string
+   = match a with
+      | [] -> []
+      | hd::tl -> string_of_int hd :: (list_int_to_list_string tl)
+
+ let main = //let f0 = Var 0 in
+//            let f1 = Var 1 in
+//            let f2 = Var 2 in
+//            let f3 = Var 3 in 
+         //   let var_for_rule_0 = DImplies f0 f1 in
+         //   let var_for_rule_1 = Implies f0 f1 in
+         //   let var_for_rule_2 = Or f0 (And f1 f2) in
+         //   let var_for_rule_3 = Or (And f1 f2) (DImplies f0 f1) in
+         //   let var_for_rule_5 = Or f0 (Or f1 f2) in
+         //   let var_for_rule_6 = And f0 (And f1 f2) in
+         //   let var_for_rule_7 = Not (And f0 f1) in
+         //   let var_for_rule_8 = Not (Or f0 f1) in
+         //   let var_for_rule_9 = Not (Not f0) in
+         //   let test_formula = DImplies (Or f1 f2) f0 in
+         //   let out1 = FStar.Printf.sprintf "%s\n" (pretty_print test_formula) in
+            //   print_string out1;
+            //   print_string (pretty_print var_for_rule_3)
+           let start_interval = 4 in
+           let end_interval = 6 in
+           let l1 = [1;2;3;4;5;6;7;8;9;10] in
+           let interv = interval_of_list l1 2 5 in
+           print_string (concat "" (list_int_to_list_string interv))
+
