Tseitin.fst
@@ -1,0 +1,102 @@
+module Tseitin
+
+open FormulaT
+open CnfFormula
+open Utils
+open TseitinCore
+module L = FStar.List.Tot.Base
+open FStar.Classical
+
+
+let satisfiable (f:formula_t {valid_formula_t f})
+    = exists tau . L.length tau = max_var f ==> truth_value f tau
+
+
+let satisfiable_cnf_formula (rf : list (list int) {valid_cnf_formula rf})
+    = exists tau . L.length tau = max_var_cnf_formula rf ==> truth_value_cnf_formula rf tau
+
+
+let equisatisfiable (f:formula_t {valid_formula_t f}) (rf : list (list int) {valid_cnf_formula rf})
+    = satisfiable f <==> satisfiable_cnf_formula rf
+
+
+// let rec tseitin_cnf (f:formula_t) (n:nat) (start_interval:nat)
+//     : Pure ((list (list int)) & int & nat)
+//            (requires n <= start_interval)
+//            (ensures fun (rf, v, end_interval) -> (valid f rf v n start_interval end_interval /\
+//                                                   tseitin_same_value f rf v n start_interval end_interval /\
+//                                                   tseitin_can_extend f rf v n start_interval end_interval))
+//     = match f with
+//         | Or f1 f2 ->
+//             let rf1, v1, mid = tseitin_cnf f1 n start_interval in
+//             let rf2, v2, v = tseitin_cnf f2 n mid in
+//             let end_interval = v + 1 in
+//             let rf = L.append (L.append rf1 rf2) (or_clauses v1 v2 v) in
+//             //proveCanExtendOr(f1, rf1, v1, f2, rf2, v2, n, start, mid, v, end, rf);
+//             //proveSameValueOr(f1, rf1, v1, f2, rf2, v2, n, start, mid, v, end, rf);
+//             rf, v, end_interval
+//         | And f1 f2 -> 
+//             let rf1, v1, mid = tseitin_cnf f1 n start_interval in
+//             let rf2, v2, v = tseitin_cnf f2 n mid in
+//             let end_interval = v + 1 in
+//             let rf = L.append (L.append rf1 rf2) (and_clauses v1 v2 v) in
+//             //proveCanExtendAnd(f1, rf1, v1, f2, rf2, v2, n, start, mid, v, end, rf);
+//             //proveSameValueAnd(f1, rf1, v1, f2, rf2, v2, n, start, mid, v, end, rf);
+//             rf, v, end_interval
+//         | Implies f1 f2 ->
+//             let rf1, v1, mid = tseitin_cnf f1 n start_interval in
+//             let rf2, v2, v = tseitin_cnf f2 n mid in
+//             let end_interval = v + 1 in
+//             let rf = L.append (L.append rf1 rf2) (implies_clauses v1 v2 v) in
+//             // proveCanExtendImplies(f1, rf1, v1, f2, rf2, v2, n, start, mid, v, end, rf);
+//             //proveSameValueImplies(f1, rf1, v1, f2, rf2, v2, n, start, mid, v, end, rf);
+//             rf, v, end_interval
+//         | DImplies f1 f2 ->
+//             let rf1, v1, mid = tseitin_cnf f1 n start_interval in
+//             let rf2, v2, v = tseitin_cnf f2 n mid in
+//             let end_interval = v + 1 in
+//             let rf = L.append (L.append rf1 rf2) (dimplies_clauses v1 v2 v) in 
+//             //proveCanExtendDimplies(f1, rf1, v1, f2, rf2, v2, n, start, mid, v, end, rf);
+//             //proveSameValueDimplies(f1, rf1, v1, f2, rf2, v2, n, start, mid, v, end, rf);
+//             rf, v, end_interval
+//         | Not f1 ->
+//             let rf1, v1, v = tseitin_cnf f1 n start_interval in
+//             let end_interval = v + 1 in
+//             let rf = L.append rf1 (not_clauses v1 v) in
+//             // proveCanExtendNot(f1, rf1, v1, n, start, v, end, rf);
+//             //proveSameValueNot(f1, rf1, v1, n, start, v, end, rf);
+//             rf, v, end_interval
+//         | Var value ->
+//             let rf = [] in
+//             let v = value in
+//             let end_interval = start_interval in
+//             let aux (tau : list bool) : Lemma (requires L.length tau = n)
+//                                               (ensures can_extend tau f rf v n start_interval end_interval)
+//                 = let tau' = L.append tau (n_falses (end_interval - n)) in
+//                   assert (L.length tau' = end_interval)
+//                 //   assert (can_extend tau f rf v n start_interval end_interval)
+//             in
+//             forall_intro (move_requires aux);
+//             assert (tseitin_can_extend f rf v n start_interval end_interval);
+//             assert (tseitin_same_value f rf v n start_interval end_interval);
+//             rf, v, end_interval
+
+// let tseitin (f:formula_t)
+//     : Pure (list (list int)) (requires valid_formula_t f)
+//                              (ensures fun r -> (valid_cnf_formula r /\ equisatisfiable f r))
+//     = let n = max_var f in
+
+
+//  method tseitin(f : FormulaT) returns (result : seq<seq<int>>)
+//         requires validFormulaT(f);
+//         ensures validCnfFormula(result);
+//         ensures equiSatisfiable(f, result);
+//     {
+//         var n := maxVar(f);
+//         var v : int;
+//         var end : int;
+//         var rf : seq<seq<int>>;
+//         rf, v, end := tseitinCnf(f, n, n);
+//         result := rf + [[posVarToLit(v)]];
+//         tseitinFollows(f, rf, v, n, end);
+//     }
