TseitinProofs.fst
@@ -1,0 +1,92 @@
+module TseitinProofs
+
+open CnfFormula
+open FormulaT
+open Utils
+open TseitinCore
+module L = FStar.List.Tot.Base
+open FStar.Classical
+
+
+let prove_same_value_not (f1:formula_t) (rf1 : list (list int)) (v1:int) (n:nat)
+                         (start_interval:nat) (end_interval:nat) (rf : list (list int)) (v:int)
+    : Lemma (requires n <= start_interval /\ start_interval <= v /\
+                      valid f1 rf1 v1 n start_interval v /\
+                      tseitin_same_value f1 rf1 v1 n start_interval v /\
+                      rf = L.append rf1 (not_clauses v1 v) /\ end_interval = v + 1)
+            (ensures valid (Not f1) rf v n start_interval end_interval /\
+                     tseitin_same_value (Not f1) rf v n start_interval end_interval)
+    = assert (valid (Not f1) rf v n start_interval end_interval);
+      let aux (tau : list bool) : Lemma (requires L.length tau >= end_interval /\
+                                                  truth_value_cnf_formula rf tau)
+                                        (ensures truth_value_literal (pos_var_to_lit v) tau = truth_value (Not f1) tau)
+          = variables_up_to_monotone f1 n (L.length tau);
+            assert (truth_value_literal (pos_var_to_lit v1) tau = truth_value f1 tau);
+            //lemma_not_clauses v1 v tau
+            assert (truth_value_literal (pos_var_to_lit v) tau = truth_value (Not f1) tau)
+      in
+      forall_intro (move_requires aux)
+
+
+let prove_can_extend_not (f1:formula_t) (rf1 : list (list int)) (v1:int) (n:nat)
+                         (start_interval:nat) (end_interval:nat) (rf : list (list int)) (v:int)
+    : Lemma (requires n <= start_interval /\ start_interval <= v /\ v < end_interval /\
+                      valid f1 rf1 v1 n start_interval v /\
+                      tseitin_can_extend f1 rf1 v1 n start_interval v /\
+                      rf = L.append rf1 (not_clauses v1 v) /\ end_interval = v + 1)
+            (ensures valid (Not f1) rf v n start_interval end_interval /\
+                     tseitin_can_extend (Not f1) rf v n start_interval end_interval)
+    = assert (n <= v);
+      assert (valid (Not f1) rf v n start_interval end_interval);
+      let aux (tau : list bool) : Lemma (requires L.length tau = n)
+                                        (ensures can_extend tau (Not f1) rf v n start_interval end_interval)
+          = assert (can_extend tau f1 rf1 v1 n start_interval v);
+            assert (valid_literal (pos_var_to_lit v1))
+
+// lemma proveCanExtendNot(f1 : FormulaT, rf1 : seq<seq<int>>, v1 : int,
+//         n : int, start : int, v : int,
+//         end : int, rf : seq<seq<int>>)
+//         requires 0 <= n <= start <= v < end;
+//         requires valid(f1, rf1, v1, n, start, v);
+//         requires tseitinCanExtend(f1, rf1, v1, n, start, v);
+//         requires rf == rf1 + notClauses(v1, v);
+//         requires end == v + 1;
+//         ensures valid(Not(f1), rf, v, n, start, end);
+//         ensures tseitinCanExtend(Not(f1), rf, v, n, start, end);
+//     {
+//         assert 0 <= n <= v;
+//         assert valid(Not(f1), rf, v, n, start, end);
+//         forall tau : seq<bool> | |tau| == n
+//             ensures canExtend(tau, Not(f1), rf, v, n, start, end);
+//         {
+//             assert canExtend(tau, f1, rf1, v1, n, start, v);
+//             assert validLiteral(posVarToLit(v1));
+
+//             ghost var tau1 :|
+//                 tau <= tau1 &&
+//                 |tau1| == v &&
+//                 truthValueCnfFormula(rf1, tau1) &&
+//                 truthValue(f1, tau) ==
+//                 truthValueLiteral(posVarToLit(v1), tau1);
+
+//             negateLiteral(v1, tau1);
+
+//             ghost var tau' := combine1(tau, tau1, n, start, v,
+//                 truthValue(Not(f1), tau));
+
+//             assert tau <= tau';
+//             assert |tau'| == end;
+//             transferTruthValue(rf1, tau1, tau', n, start, v);
+
+//             transferTruthValueLit(posVarToLit(v1), tau1, tau', n, start, v);
+//             assert truthValueLiteral(posVarToLit(v1), tau') ==
+//                 truthValue(f1, tau);
+//             transferTruthValueLit(negVarToLit(v1), tau1, tau', n, start, v);
+//             assert truthValueLiteral(negVarToLit(v1), tau1) ==
+//                 !truthValueLiteral(posVarToLit(v1), tau1);
+
+//             lemmaNotClauses(v1, v, tau');
+
+//             assert truthValueCnfFormula(rf, tau');
+//         }
+//     }
